Test.Float/Test.Float.Ranges.fst
@@ -1,0 +1,69 @@
+module Test.Float.Ranges
+
+open Test.Float.Base
+open Test.Float.Lemmas.Arithmetic
+open Test.Float.Lemmas.Inequality
+
+type endpoint =
+  | Opened: p:float -> endpoint
+  | Closed: p:float -> endpoint
+
+let v point =
+  match point with
+  | Opened p -> p
+  | Closed p -> p
+
+let satisfy {| binrel_pair |} x point =
+  match point with
+  | Opened p -> x <??> p
+  | Closed p -> x <?=> p
+
+let (>^) = satisfy #weak_gt
+let (<^) = satisfy #weak_lt
+
+let (>.<) {| binrel_pair |} p1 p2 =
+  match p1, p2 with
+  | Closed v1, Opened v2 -> v1 <??> v2
+  | _, _ -> v p1 <?=> v p2
+
+let (>>.<) = (>.<) #weak_gt
+let (>.<<) = (>.<) #weak_lt
+
+let commut_endpoint {| binrel_pair |} (a b c: endpoint) : Lemma
+  (requires a >.< b /\ b >.< c)
+  (ensures a >.< c)
+  =
+  match a, b, c with
+  | Closed _, Opened _,        _ -> commut_binrel_left (v a) (v b) (v c)
+  |        _, Closed _, Opened _ -> commut_binrel_right (v a) (v b) (v c)
+  |        _,        _,        _ -> binrel_commut_weak (v a) (v b) (v c)
+
+
+
+type range = { l: endpoint; r: endpoint }
+
+let ( |-> ) x (rng: range) = x >^ rng.l /\ x <^ rng.r
+
+let (<.|> ) x (left, right) = x |-> { l = (Closed left); r = (Opened right) }
+let ( <|.>) x (left, right) = x |-> { l = (Opened left); r = (Closed right) }
+let (<.|.>) x (left, right) = x |-> { l = (Closed left); r = (Closed right) }
+let ( <|> ) x (left, right) = x |-> { l = (Opened left); r = (Opened right) }
+
+let ( |=> ) (less more: range) =
+  less.l >>.< more.l /\
+  less.r >.<< more.r
+
+let single (x: float) : Pure range (requires True) 
+  (ensures fun range -> x |-> range /\ (forall (y: float{y |-> range}). y = x)) =
+  { l = Closed x; r = Closed x }
+
+let contains_is_closed_range range x : Lemma (x |-> range <==> single x |=> range) = ()
+
+let range_inj (a b c: range) : Lemma (requires a |=> b /\ b |=> c) (ensures a |=> c) =
+  commut_endpoint #weak_gt a.l b.l c.l;
+  commut_endpoint #weak_lt a.r b.r c.r;
+  assert (a.l >>.< c.l);
+  assert (a.r >.<< c.r)
+
+let point_inj x a b : Lemma (requires x |-> a /\ a |=> b) (ensures x |-> b) =
+  range_inj (single x) a b
